Treat Iff hyps as equations
- Do not split hypotheses of type `P ↔ Q`.
- Extend the builtin subst rule such that it recognises hyps `P ↔ Q` and
  treats them as equalities `P = Q`. (The simplifier already does this.)
- Bonus: register a builtin simp rule which rewrites morally-homogeneous
  equations (`@HEq α x α y`) into actually-homogeneous equations
  (`@Eq α x y`). This means such equations are also picked up by the
  subst rule. (Lean's `subst` tactic also recognises such heterogeneous
  equations.)

Aesop/BuiltinRules/Subst.lean
@@ -12,6 +12,31 @@ open Std (HashSet)
 
 namespace Aesop.BuiltinRules
 
+private def iffToEq (goal : MVarId) (fvarId : FVarId) (lhs : Expr)
+    (rhs : Expr) : MetaM (MVarId × FVarId) := do
+  let newType ← mkEq lhs rhs
+  let proof ← mkPropExt (.fvar fvarId)
+  let goal ← goal.assert (← fvarId.getUserName) newType proof
+  let (newFVarId, goal) ← goal.intro1P
+  let goal ← goal.tryClear fvarId
+  return (goal, newFVarId)
+
+-- If the `fvarId` is an `Iff`, it is turned into an `Eq`. If the `fvarId` is an
+-- `Eq`, it is returned unchanged. Additionally, the type, LHS and RHS of the
+-- resulting equation are returned.
+private def prepareSubstHyp (goal : MVarId) (fvarId : FVarId) :
+    MetaM (Option (MVarId × FVarId × Expr × Expr × Expr)) :=
+  goal.withContext do
+    let ty ← instantiateMVars $ ← fvarId.getType
+    matchHelper? ty λ ty => do
+      if let some (α, lhs, rhs) := ty.eq? then
+        return some (goal, fvarId, α, lhs, rhs)
+      else if let some (lhs, rhs) := ty.iff? then
+        let (goal, fvarId) ← iffToEq goal fvarId lhs rhs
+        return some (goal, fvarId, .sort .zero, lhs, rhs)
+      else
+        return none
+
 partial def substFVars (goal : MVarId) (fvarIds : Array FVarId) :
     MetaM (Option (MVarId × FVarSubst)) := do
   let (goal, modified, fvarSubst) ← go 0 false {} goal
@@ -23,11 +48,14 @@ partial def substFVars (goal : MVarId) (fvarIds : Array FVarId) :
         if h : i < fvarIds.size then
           let (.fvar fvarId) := fvarSubst.get $ fvarIds.get ⟨i, h⟩ | throwError
             "unexpected expr in FVarSubst"
-          let type ← instantiateMVars (← fvarId.getDecl).type
-          let (some (_, lhs, _)) ← matchEq? type
+          let some (goal, fvarId', _, lhs, _) ← prepareSubstHyp goal fvarId
             | go (i + 1) modified fvarSubst goal
-          let symm := ! lhs.isFVar
-          match ← substCore? goal fvarId (symm := symm) fvarSubst with
+          let fvarSubst :=
+            if fvarId' == fvarId then
+              fvarSubst
+            else
+              fvarSubst.insert fvarId (.fvar fvarId')
+          match ← substCore? goal fvarId' (symm := ! lhs.isFVar) fvarSubst with
           | none =>
             go (i + 1) modified fvarSubst goal
           | some (fvarSubst, goal) =>
@@ -36,16 +64,12 @@ partial def substFVars (goal : MVarId) (fvarIds : Array FVarId) :
           return (goal, modified, fvarSubst)
 
 @[aesop (rule_sets [builtin]) norm -50
-  (tactic (uses_branch_state := false) (index := [hyp _ = _]))]
-def subst : RuleTac := λ input => do
+  (tactic (uses_branch_state := false) (index := [hyp _ = _, hyp _ ↔ _]))]
+def subst : RuleTac := SimpleRuleTac.toRuleTac λ input => do
   let hyps ← input.indexMatchLocations.toArray.mapM λ
     | .hyp ldecl => pure ldecl.fvarId
     | _ => throwError "unexpected index match location"
   let (some (goal, _)) ← substFVars input.goal hyps | throwError
     "no suitable hypothesis found"
-  let postState ← saveState
-  return {
-    applications := #[{ goals := #[goal], postState }],
-    postBranchState? := none
-  }
+  return [goal]
 end Aesop.BuiltinRules
