tests/run/Subst.lean
@@ -11,10 +11,50 @@ set_option aesop.check.all true
 -- These test cases test the builtin subst tactic.
 
 example (h₁ : x = 5) (h₂ : y = 5) : x = y := by
-  aesop
+  fail_if_success
+    aesop
+      (erase Aesop.BuiltinRules.subst)
+      (simp_options := { useHyps := false })
+      (options := { terminal := true })
+  aesop (simp_options := { useHyps := false })
 
 example (h₁ : x = y) (h₂ : y = z) : x = z := by
-  aesop
+  fail_if_success
+    aesop
+      (erase Aesop.BuiltinRules.subst)
+      (simp_options := { useHyps := false })
+      (options := { terminal := true })
+  aesop (simp_options := { useHyps := false })
 
 example (P : ∀ x y, x = y → Prop) (h₁ : x = y) (h₂ : P x y h₁) : x = y := by
+  fail_if_success
+    aesop
+      (erase Aesop.BuiltinRules.subst,
+             Aesop.BuiltinRules.assumption,
+             Aesop.BuiltinRules.applyHyps)
+      (simp_options := { useHyps := false })
+      (options := { terminal := true })
   aesop
+    (erase Aesop.BuiltinRules.assumption,
+           Aesop.BuiltinRules.applyHyps)
+    (simp_options := { useHyps := false })
+
+-- Subst also works for bi-implications.
+example (h₁ : P ↔ Q) (h₂ : Q ↔ R) (h₃ : P) : R  := by
+  fail_if_success
+    aesop
+      (erase Aesop.BuiltinRules.subst)
+      (simp_options := { useHyps := false })
+      (options := { terminal := true })
+  aesop (simp_options := { useHyps := false })
+
+-- Subst also works for morally-homogeneous heterogeneous equalities (using a
+-- builtin simp rule which turns these into actual homogeneous equalities).
+example {P : α → Prop} {x y z : α} (h₁ : HEq x y) (h₂ : HEq y z) (h₃ : P x) :
+    P z  := by
+  fail_if_success
+    aesop
+      (erase Aesop.BuiltinRules.subst)
+      (simp_options := { useHyps := false })
+      (options := { terminal := true })
+  aesop (simp_options := { useHyps := false })
